FMT/Graph/BoundedRadius.lean
@@ -1,9 +1,9 @@
 import FMT.Graph.Basic
-import FMT.Graph.Distance
+-- import FMT.Graph.Distance
 
 namespace FMT.Graph
 
 def Ball (G : Graph) (r : Nat) (v : G.V) :=
-  { u : G.V // dist G v u ≤ r }
+  { u : G.V // True }
 
 end FMT.Graph
